day1/ast.fsti
@@ -1,0 +1,31 @@
+module Ast
+
+type infer : Type = 
+    | Infer     : infer
+
+type check = 
+    | Check     : check
+
+type term       : Type -> Type = 
+    | Annoted   : term check -> typeL -> term infer
+    | Bound     : nat -> term infer
+    | Free      : name -> term infer
+    | Apply     : term infer -> term check -> term infer
+    | Inferable : term infer -> term check
+    | Lambda    : term check -> term check
+
+and name        : Type = 
+    | Global    : string -> name
+    | Local     : nat -> name
+    | Quote     : nat -> name
+
+and typeL       : Type = 
+    | TFree     : name -> typeL
+    | Function  : typeL -> typeL -> typeL
+
+type kindL      : Type = 
+    | Star      : kindL
+
+type info       : Type =
+    | HasKind   : kindL -> info
+    | HasType   : typeL -> info
