day1/checker.fsti
@@ -1,0 +1,12 @@
+module Checker
+
+open Try
+open Ast
+
+type context    : Type = list (name * info)
+
+val size : (#a:Type) -> term a -> nat
+
+val typeInfer   : nat -> context -> (e:term infer) -> Tot (result typeL) (decreases (size e))
+val typeCheck   : nat -> context -> (e:term check) -> (t:typeL) -> Tot (result unit) (decreases %[size e;t])
+val typeInfer0  : context -> term infer -> result typeL
