day1/closed.fst
@@ -1,0 +1,12 @@
+module Closed
+
+open Try
+open Ast
+
+let rec closed l = function
+    | Annoted e t -> closed l e
+    | Bound j     -> if List.mem j l then return () else throwError "unbound variable"
+    | Free x      -> return ()
+    | Apply e1 e2 -> closed l e1 >>= (fun _ -> closed l e2)
+    | Inferable e -> closed l e
+    | Lambda e    -> closed l e
