day1/closed.fsti
@@ -1,0 +1,7 @@
+module Closed
+
+open Try
+open Ast
+
+val closed : (#a:Type) -> list nat -> e:term a -> Tot (result unit) (decreases e)
+
