day1/eval.fsti
@@ -1,0 +1,16 @@
+module Eval
+
+open Ast
+
+type value : Type =
+    | Value : value
+
+type neutral : Type =
+    | Neutral : neutral
+
+type vterm      : Type -> Type =
+    | VLam      : nat -> vterm value -> vterm value
+    | VNeutral  : vterm neutral -> vterm value
+    | NFree     : name -> vterm neutral
+    | NApp      : vterm neutral -> vterm value -> vterm neutral
+
