day1/try.fst
@@ -1,0 +1,18 @@
+module Try
+
+let return = Inr
+
+let throwError = Inl
+
+let (<$>) f =
+    function
+    | Inl s -> throwError s
+    | Inr a -> return (f a)
+
+let (>>=) r f =
+    match r with
+    | Inl s -> throwError s
+    | Inr a -> f a
+
+let unless r f e = 
+    r >>= (fun r -> if f r then return r else e)
