day1/try.fsti
@@ -1,0 +1,9 @@
+module Try
+
+type result a : Type = either string a
+
+val return     : (#a:Type) -> a -> Tot (result a)
+val throwError : (#a:Type) -> string -> Tot (result a)
+val (<$>)      : (#a:Type) -> (#b:Type) -> (a -> b) -> result a -> Tot (result b)
+val (>>=)      : (#a:Type) -> (#b:Type) -> result a -> (a -> result b) -> Tot (result b)
+val unless     : (#a:Type) -> result a -> (a -> bool) -> result a -> Tot (result a)
