day1/utils.fst
@@ -1,0 +1,3 @@
+module Utils
+
+let constant b _ = b
