day1/utils.fsti
@@ -1,0 +1,3 @@
+module Utils
+
+val constant    : (#a:Type) -> (#b :Type) -> b -> a -> Tot b
